theories/typechecker.v
@@ -1,0 +1,534 @@
+From det Require Import prelude.
+From mathcomp Require Import all_ssreflect.
+From det Require Import tree tree_prop ctx tree_vars unif mut_excl fresh sig_lattice sig_compat.
+From elpi.apps Require Import derive derive.std.
+From HB Require Import structures.
+
+
+Definition cincl s1 s2 := compat_type s1 s2 && incl s1 s2.
+
+Lemma cincl_weakr t1 t2: cincl t1 t2 -> cincl t1 (weak t2).
+Proof. by rewrite/cincl => /andP[C1 I1]; rewrite compat_type_weak incl_weakr//C1. Qed.
+
+Lemma cincl_weakrR t1 t2: compat_type t1 t2 -> cincl t1 (weak t2).
+Proof. by rewrite/cincl => C1; rewrite compat_type_weak C1 compat_type_incl_weak//. Qed.
+
+Lemma cincl_weakeq t1 t2: cincl t1 t2 -> (weak t1) = (weak t2).
+Proof. by move=> /andP[/compat_type_weak_eq]. Qed.
+
+Lemma deref_in (s:Sigma) (v:V) (vs : v \in s): idempotent s -> deref s s.[vs] = s.[vs].
+Proof. by move=> A; have:= deref2 (Tm_V v) A; rewrite/=in_fnd. Qed.
+
+Lemma cinclR_min C A B: cincl C A -> cincl C B -> cincl C (min A B) .
+Proof.
+  rewrite/cincl => /andP[cca ica] /andP[ccb icb].
+  rewrite inclR_min// andbT.
+  apply/compat_type_trans/compat_type_minR => //.
+  by apply/compat_type_trans/ccb; rewrite compat_type_comm.
+Qed.
+
+Lemma cinclL_min C A B: compat_type A B -> (cincl B C || cincl A C) -> cincl (min A B) C.
+Proof.
+  move=> cab /orP[]/andP[C1 I1]; rewrite /cincl; apply/andP; split.
+    by rewrite compat_type_comm min_comm; apply/compat_type_trans/compat_type_minR; rewrite compat_type_comm.
+    by rewrite min_comm inclL_min.
+    by rewrite compat_type_comm; apply/compat_type_trans/compat_type_minR; rewrite//compat_type_comm.
+  by rewrite inclL_min.
+Qed.
+
+Definition sigV := {fmap V -> S}.
+
+Definition is_sigV (x : sigV) := unit.
+Lemma is_sigV_inhab : forall x, is_sigV x. Proof. exact (fun x => tt). Qed.
+Definition sigV_eqb (x y : sigV) := x == y.
+Lemma sigV_eqb_correct : forall x, eqb_correct_on sigV_eqb x. Proof. by move=>??/eqP. Qed.
+Lemma sigV_eqb_refl : forall x, eqb_refl_on sigV_eqb x. Proof. by move=>?; exact: eqxx. Qed.
+Elpi derive.eqbOK.register_axiomx sigV is_sigV is_sigV_inhab sigV_eqb sigV_eqb_correct sigV_eqb_refl.
+HB.instance Definition _ : hasDecEq sigV := Equality.copy sigV _.
+
+
+Definition odflt1 {T} (ab : T * bool) x := 
+  match x with (Some x, b1) => (x,b1) | (None,_) => ab end.
+
+Definition flex_head T := if get_tm_hd T is inr _ then true else false.
+
+Lemma cincl_trans : transitive cincl.
+Proof. by move=> x y z /andP[C1 I1] /andP[C2 I2]; rewrite /cincl (incl_trans I1 I2) (compat_type_trans C1 C2). Qed.
+
+Lemma cincl_refl: reflexive cincl.
+Proof. by rewrite /cincl/reflexive => x; rewrite compat_type_refl incl_refl. Qed.
+
+Hint Resolve cincl_refl : core.
+
+Lemma cincl_arr m m' a b a' b':
+  cincl (arr m a b) (arr m' a' b') =
+    [&& m' == m, (if m == input then cincl a' a else cincl a a') & cincl b b'].
+Proof.
+  rewrite/cincl/=; case: m; case: m' => //; rewrite incl_arr/= -!andbA; f_equal.
+    by apply: compat_type_comm.
+    by case: compat_type => //; rewrite andbF.
+  by case: compat_type => //=; rewrite andbF.
+Qed.
+
+Lemma cincl_is_det_sig a b: cincl a b ->  is_det_sig b ->  is_det_sig a.
+Proof.
+  elim: a b => //=[|m f Hf a Ha]//=.
+    by move=> [|[]]//=[[|[]]|[]]//=.
+  case: m => -[|[]]//f' a'; rewrite cincl_arr/= => /andP[] _ /Ha; auto.
+Qed.
+
+Fixpoint typechecks (sP : sigT) (sV : sigV) (tm : Tm) : option (sigV * S) :=
+let map_sV := omap (pair sV) in
+match tm with
+| Tm_V v => map_sV sV.[?v]
+| Tm_P p => map_sV sP.[?p]
+| Tm_App h bo =>
+  match typechecks sP sV h with
+  | None => None
+  | Some (sV, (arr m l r)) =>
+      match typechecks sP sV bo with
+      | None => 
+        if bo is Tm_V v then Some (sV.[v <- weak l], r)
+        else None
+      | Some (sV, tyb) => 
+        if compat_type tyb l then Some (sV, r)
+        else None
+      end
+  | _ => None
+  end
+end.
+
+Lemma typechecks_cat sP g t r:
+  typechecks sP g t = Some r -> exists x : sigV, r.1 = x + g.
+Proof.
+  elim: t g r => [p|v|f Hf a Ha] g r/=; only 1, 2: by case: fndP => //pP[<-]; exists fmap0; rewrite cat0f.
+  case TF: typechecks => [[gf [|m tf ta]]|]//.
+  have /=[xf {}Hf] := Hf _ _ TF; subst.
+  case TA: typechecks => [[ga tb]|].
+    case: ifP => //CT[<-{r}].
+    have /=[xa {}Ha] := Ha _ _ TA; subst.
+    by exists (xa + xf); rewrite catfA.
+  case: a TA {Ha} => //v.
+  rewrite/typechecks fnd_cat/=; case: fndP => vg//=.
+  case: fndP => //=vx _ [<-{r}]/=. 
+  exists (xf.[v<-weak tf]).
+  rewrite setf_catl; f_equal.
+  apply/fmapP => k; rewrite fnd_rem in_fset1; case: eqP => ?//; subst.
+  by rewrite not_fnd.
+Qed.
+
+Lemma typechecks_covers sP g g' t s:
+  typechecks sP g t = Some (g', s) ->
+  [forall x : vars t, val x \in domf g'].
+Proof.
+  move=> H; apply/forallP => -[]/=.
+  elim: t g g' s H => [p|v|f Hf a Ha] g g' s//=.
+    move=> H v'; rewrite in_fset1 => /eqP?; subst.
+    by move: H; case: fndP => //=? [<-].
+  have:= Hf g; case TF: typechecks => [[gf [|m tf ta]]|]//.
+  move=> /(_ _ _ erefl){}Hf.
+  have:= Ha gf; case TA: typechecks => [[ga tb]|]//.
+    move=> /(_ _ _ erefl){}Ha; case: ifP => //CT[<-{g'}?]; subst.
+    move=> v; rewrite in_fsetU => /orP[/Hf|/Ha]//.
+    have [x/=->] := typechecks_cat TA.
+    by apply/fsubsetP; rewrite domf_cat fsubsetUr.
+  move=> _; case: a {Ha} TA => //=v; case: fndP => //vgf _ [<-{g'}?]; subst.
+  by move=> v'; rewrite /= !in_fsetU !in_fset1 orbC; case: eqP => //=vv; eauto.
+Qed.
+
+Lemma typechecks_app sP sV f a: 
+  typechecks sP sV (Tm_App f a) =
+    match typechecks sP sV f with
+  | None => None
+  | Some (sV, (arr m l r)) =>
+      match typechecks sP sV a with
+      | None => 
+        if a is Tm_V v then Some (sV.[v <- weak l], r)
+        else None
+      | Some (sV, tyb) => 
+        if compat_type tyb l then Some (sV, r)
+        else None
+      end
+  | _ => None
+  end.
+Proof. by []. Qed.
+
+Lemma typechecks_P sP sV p: 
+  typechecks sP sV (Tm_P p) = omap (pair sV) sP.[?p].
+Proof. by []. Qed.
+
+Lemma typechecks_V sP sV v: 
+  typechecks sP sV (Tm_V v) = omap (pair sV) sV.[?v].
+Proof. by []. Qed.
+
+Definition simpl_typechecks := (typechecks_app, typechecks_P, typechecks_V).
+
+Definition is_prop t : option sigV := match t with Some (sV, b (d _)) => Some sV | _ => None end.
+
+Definition typechecks_atom sP sV a : option sigV :=
+match a with
+| call t => is_prop (typechecks sP sV t)
+| _ => Some sV
+end.
+
+Fixpoint typechecks_atoms sP g atoms :=
+match atoms with
+| [::] => Some g
+| x :: xs => obind (fun g => typechecks_atoms sP g xs) (typechecks_atom sP g x)
+end.
+
+Lemma typecheck_atoms_cons sP g x xs:
+  typechecks_atoms sP g (x :: xs) = obind (fun g => typechecks_atoms sP g xs) (typechecks_atom sP g x).
+Proof. by []. Qed.
+
+Definition typechecks_rule sP (r : R) := 
+  typechecks_atoms sP fmap0 (call r.(head) :: r.(premises)).
+
+Module spec.
+  Fixpoint typecheck (sP : sigT) (sV : sigV) (tm : Tm) : option S :=
+  match tm with
+  | Tm_V v => sV.[?v]
+  | Tm_P p => sP.[?p]
+  | Tm_App h bo =>
+    match typecheck sP sV h with
+    | None => None
+    | Some (arr m l r) =>
+        match typecheck sP sV bo with
+        | None => None
+        | Some tyb => if compat_type tyb l then Some r else None
+        end
+    | _ => None
+    end
+  end.
+
+  Lemma typecheck_cat sP g t r k:
+    typecheck sP (k + g) t = Some r ->
+      typecheck sP g t = Some r \/ typecheck sP g t = None.
+  Proof.
+    elim: t r => [p/=|v|/=f Hf a Ha] r.
+      by case: fndP => //pP[<-{r}]; left.
+      rewrite /typecheck fnd_cat; case: fndP => vg; last by right.
+      by move=> [<-]; left.
+    case TF: typecheck => [[|m tf ta]|]//.
+    case TA: typecheck => [tb|]//.
+    case: ifP => // C [<-{r}].
+    have{Hf}:= Hf _ TF => -[]->; last by right.
+    have{Ha}:= Ha _ TA => -[]->; last by right.
+    by rewrite C; left.
+  Qed.
+
+  Lemma typecheck_catN sP g t k:
+    typecheck sP (k + g) t = None -> typecheck sP g t = None.
+  Proof.
+    elim: t => [p/=|v|/=f + a +].
+      by case: fndP => //pP[<-{r}]; left.
+      by rewrite /typecheck fnd_cat; case: fndP => vg//.
+    case TF: typecheck => [t|]//; last by move=> ->.
+    case: (typecheck_cat TF) => ->// _.
+    case: t {TF} => // _ tf ta.
+    case TA: typecheck => [t'|]; last by move=> ->.
+    case: (typecheck_cat TA) => ->//.
+  Qed.
+
+  Lemma typecheck_cat1 sP g t r k:
+    typecheck sP g t = Some r ->
+    typecheck sP (k + g) t = Some r.
+  Proof.
+    elim: t r => [p/=|v|/=f Hf a Ha] r.
+      by case: fndP => //.
+      by rewrite /typecheck fnd_cat; case: fndP.
+    case TF: typecheck => [[|m tf ta]|]//.
+    case TA: typecheck => [tb|]//.
+    case: ifP => // C [<-{r}].
+    by rewrite (Hf _ TF) (Ha _ TA) C.
+  Qed.
+  
+  Lemma typechecks_correct sP g tm:
+    match typechecks sP g tm with
+    | None => typecheck sP g tm = None
+    | Some (g,s) => typecheck sP g tm = Some s
+    end.
+  Proof.
+    elim: tm g => [p|v|f Hf a Ha] g//=.
+      by case: fndP => //.
+      by case: fndP => //=vg; rewrite in_fnd.
+    have{Hf}:= Hf g; case TF: typechecks => [[gf tf]|]//=; last by move=>->.
+    have [xf/= ?] := typechecks_cat TF; subst.
+    case: tf TF => [err|m tf ta] TF TF'.
+      by have:= typecheck_cat TF' => -[]->//.
+    move: {Ha} (Ha (xf + g)).
+    case TA: typechecks => [[ga tb]|] TA'.
+      have [xa/= ?] := typechecks_cat TA; subst.
+      case: ifP => CT.
+        by rewrite (typecheck_cat1 _ TF') TA' CT.
+      case: (typecheck_cat TF') => ->//.
+      rewrite catfA in TA'.
+      by case: (typecheck_cat TA') => ->//; rewrite CT.
+    case V: (is_var a).
+      case: a V TA TA' => //v _.
+      rewrite/typechecks{1}/typecheck fnd_cat.
+      case: fndP => // vgf.
+      case: fndP => //vxf _ _.
+      rewrite {2}/typecheck fnd_set eqxx/= cat_set_eq disjoint_catfC.
+        by rewrite (typecheck_cat1 _ TF') compat_type_weak compat_type_refl.
+      by rewrite domf_cat/= fsetU0 fdisjointX1 in_fsetU (negbTE vxf)//.
+    set X := (match a with Tm_V _ => _ | _ => _ end).
+    replace X with (@None (sigV * S)); last by destruct a.
+    case: (typecheck_cat TF') => ->//{X}.
+    by rewrite (typecheck_catN TA').
+Qed.
+End spec.
+
+Definition typechecks_rules (s : sigT) (rs: seq R) :=
+  all (typechecks_rule s) rs.
+
+Definition typechecks_prog p := typechecks_rules p.(sig) p.(rules).
+
+Module Test.
+  Local Notation p := (b (d Pred)).
+  Local Notation f := (b (d Func)).
+  Local Notation e := (b Exp).
+  Local Notation V1 := (IV 0).
+  Local Notation V2 := (IV 1).
+  Local Notation F := (IV 2).
+
+  Local Definition mkP sym sig r := {| sig := [fmap].[sym <- sig]; rules := [::r] |}.
+
+  Module Once.
+    Notation onceSym := (IP 1).
+    Definition onceI   := mkR (Tm_App (Tm_P onceSym) (Tm_V V1)) [::call (Tm_V V1); cut].
+    Definition onceSig := arr input p f.
+
+    Goal typechecks_prog (mkP onceSym onceSig onceI).
+    Proof.
+      rewrite/typechecks_prog/= andbT/typechecks_rule.
+      rewrite !typecheck_atoms_cons/typechecks_atom !simpl_typechecks.
+      rewrite !FmapE.fmapE eqxx/onceSig [omap _ _]/=.
+      cbn match. rewrite simpl_typechecks not_fnd// [omap _ _]/=.
+      cbn match; rewrite/Option.bind/oapp/is_prop.
+      rewrite typecheck_atoms_cons/typechecks_atom simpl_typechecks !FmapE.fmapE.
+      by rewrite eqxx.
+    Qed.
+  End Once.
+  
+  Module Do.
+    Notation doSym := (IP 2).
+    Definition doI   := mkR (Tm_App (Tm_P doSym) (Tm_V V1)) [::call (Tm_V V1)].
+    Definition doSig := arr input f f.
+
+    Goal typechecks_prog (mkP doSym doSig doI).
+    Proof.
+      rewrite/typechecks_prog/= andbT/typechecks_rule.
+      rewrite !typecheck_atoms_cons/typechecks_atom !simpl_typechecks.
+      rewrite !FmapE.fmapE eqxx/doSig [omap _ _]/=.
+      cbn match. rewrite simpl_typechecks not_fnd// [omap _ _]/=.
+      cbn match; rewrite/Option.bind/oapp/is_prop.
+      rewrite typecheck_atoms_cons/typechecks_atom simpl_typechecks !FmapE.fmapE.
+      by rewrite eqxx.
+    Qed.
+  End Do.
+  
+  (* apply F X :- F X. *)
+  Module Apply.
+    Notation applySym := (IP 3).
+    Definition applyI   := mkR (Tm_App (Tm_App (Tm_P applySym) (Tm_V F)) (Tm_V V1)) [::call (Tm_App (Tm_V F) (Tm_V V1))].
+    Definition applySig := arr input (arr input e f) (arr input e f).
+
+    Goal typechecks_prog (mkP applySym applySig applyI).
+    Proof.
+      rewrite/typechecks_prog/= andbT/typechecks_rule.
+      rewrite !typecheck_atoms_cons/typechecks_atom !simpl_typechecks.
+      rewrite !FmapE.fmapE eqxx/applySig [omap _ _]/=.
+      cbn match. rewrite simpl_typechecks not_fnd// [omap _ _]/=.
+      cbn match; rewrite/Option.bind/oapp/is_prop.
+      rewrite !simpl_typechecks !FmapE.fmapE not_fnd//.
+      rewrite [omap _ _]/=; cbn match.
+      rewrite typecheck_atoms_cons/typechecks_atoms/typechecks_atom.
+      rewrite !simpl_typechecks !FmapE.fmapE eqxx [omap _ _]/=; cbn match.
+      rewrite !simpl_typechecks !FmapE.fmapE eqxx [omap _ _]/=; cbn match.
+      rewrite compat_type_refl//.
+    Qed.
+  End Apply.
+
+  Module map.
+    Local Definition map := IP 0.
+    Local Definition cons := IP 10.
+    Local Definition nil := IP 11.
+    Local Definition one := IP 12.
+    Local Definition two := IP 13.
+    Local Definition four := IP 15.
+    Local Notation app := Tm_App.
+
+    Coercion Tm_P : P >-> Tm. 
+    Coercion Tm_V : V >-> Tm. 
+
+    Local Definition prop := b (d Pred).
+    Local Definition func := b (d Func).
+    Definition exp := b Exp.
+
+    Definition mapS := arr input (arr input exp (arr output exp func)) (arr input exp (arr output exp func)).
+    Definition consS := arr input exp (arr input exp exp).
+    Definition nilS := exp.
+
+    Local Definition X := IV 1.
+    Local Definition X' := IV 10.
+    Local Definition Y := IV 2.
+    Local Definition Y' := IV 20.
+    Local Definition F := IV 3.
+
+    Local Definition p' := {|
+      sig := [fmap].[map <- mapS].[cons <- consS].[nil <- nilS];
+      rules := 
+        mkR (app (app (app map F) nil) nil) [::] ::
+        mkR (app (app (app map F) (app (app cons X) Y)) (app (app cons X') Y') ) 
+          [:: call (app (app F X) X'); call (app (app (app map F) Y) Y')] :: [::]
+    |}.
+
+    Local Lemma gthm : get_tm_hd map = inl map.
+    Proof. by []. Qed.
+
+    Ltac simpl_tc := rewrite simpl_typechecks ?FmapE.fmapE ?[omap _ _]/=; cbn match; rewrite ?compat_type_refl.
+    Ltac simpl_obind:= rewrite /Option.bind/oapp/is_prop.
+    Ltac simpl_check_atoms := rewrite typecheck_atoms_cons /typechecks_atom; repeat simpl_tc.
+
+    Local Goal typechecks_prog p'.
+    Proof.
+      rewrite/typechecks_prog/= andbT/typechecks_rule ![head _]/= ![premises _]/=.
+      apply/andP; split.
+        simpl_check_atoms; simpl_obind; repeat simpl_tc.
+        rewrite/mapS not_fnd//[omap _ _]/=; cbn match; simpl_tc.
+        by rewrite simpl_typechecks !FmapE.fmapE/=.
+      simpl_check_atoms; simpl_obind; repeat simpl_tc.
+      rewrite/mapS not_fnd// [omap _ _]/=; cbn match.
+      repeat simpl_tc.
+      rewrite/consS not_fnd// [omap _ _]/=/mapS.
+      simpl_tc; rewrite not_fnd// [omap _ _]/=; cbn match.
+      rewrite compat_type_refl; repeat simpl_tc.
+      rewrite/consS not_fnd// [omap _ _]/=/mapS.
+      repeat simpl_tc; rewrite/consS not_fnd// [omap _ _]/=/mapS.
+      rewrite compat_type_refl; repeat simpl_tc.
+      rewrite/func; simpl_check_atoms.
+      simpl_obind; simpl_check_atoms; simpl_obind.
+      rewrite [compat_type _ _]/=; cbn match.
+      by repeat simpl_tc.
+    Qed.
+  End map. 
+End Test.
+
+Definition deref_atom s a :=
+  match a with
+  | cut => cut
+  | call t => call (deref s t)
+  end.
+
+Lemma tc_bc p n t s g0 r:
+  s = fmap0 ->
+  typechecks_prog p ->
+  typechecks p.(sig) g0 (deref s t) = Some r ->
+  is_prop (Some r) ->
+  all (fun x => typechecks_atoms p.(sig) r.1 (map (deref_atom x.1) x.2)) (bc u p n t s).2.
+Proof.
+  move=> ->.
+  case: p => rs sig/=; case: r => gt [[|prop]|]// ++ _.
+  rewrite /typechecks_prog/=/bc.
+  case: ifP => // /negbFE Is; rewrite !push/=.
+  have:= idempotent_deref_disjoint t Is.
+  set dt := (deref _ _).
+  set X := fresh _; have:= leqnn X; rewrite{1}/X.
+  rewrite !freshPU freshP1 -!andbA => /and5P[Sn Sd Sc St Sp].
+  clearbody X => H + TC.
+  elim: rs Sp => //= -[h b] rs.
+  rewrite !push/= v_prog_cons !freshPU -!andbA /varsU_rhead/varsU_rprem/=.
+  move=> IH /and3P[Sh Sb Srs] /andP[Tr Trs].
+  case HH: lang.H => [[ty s']|]/=; rewrite {}IH// andbT.
+  move: HH; rewrite/fresh_rule !push/=.
+  set F := fresh_tm _ _ _.
+Abort.
+
+Fixpoint typechecks_tree sP e s t :=
+(* TODO: consider that in input I receive valid_trees *)
+match t with
+| KO | OK => Some e
+| Unexplored atom => typechecks_atom sP e (deref_atom s atom)
+| And A B0 B => 
+  obind 
+    (fun x => if typechecks_tree sP x s B && typechecks_atoms sP x (map (deref_atom s) B0)
+              then Some x else None) (typechecks_tree sP e s A)
+| Or None sm B => typechecks_tree sP e sm B
+| Or (Some A) sm B => 
+  if typechecks_tree sP e s A && typechecks_tree sP e sm B then Some e
+  else None
+end.
+
+Lemma typechecks_tree_big_and sP e s l:
+  typechecks_tree sP e s (big_and l) =
+  typechecks_atoms sP e (map (deref_atom s) l).
+Proof.
+  rewrite/big_and; case: l => //=+l.
+  elim: l e => //=[|x xs IH] e a.
+    by case: typechecks_atom.
+  case TA: typechecks_atom => [e'|]//=.
+  rewrite IH andbb.
+  case: typechecks_atom => //=?.
+  case: typechecks_atoms => //=.
+Admitted.
+
+Lemma typechecks_tree_prune sP env s t t' b:
+  typechecks_tree sP env s t ->
+  prune b t = Some t' ->
+  typechecks_tree sP env s t'.
+Proof.
+  elim_tree t b s env t' => /=.
+  - by case: b => // _ [<-].
+  - by move=> + [<-].
+  - case: ifP => ///andP[TA TB] _.
+    case PA: prune => [A'|]//=.
+      by move=> [<-{t'}]; rewrite/= TB (HA b)//.
+    case PB: prune => [B'|]//= [<-{t'}]/=.
+    by apply: (HB false).
+  - by case PB: prune => //= + [<-]/=; eauto.
+  case TA: typechecks_tree => //=[eA].
+  case: ifP => //=/andP[TB TB0] _.
+  case: ifP => //sA.
+    case PB: prune => [B'|].
+      by move=> [<-]/=; rewrite TA/= (HB b)//= TB0.
+    case PA: prune => [A'|]//=[<-]/=.
+    have:= HA _ _ _ _ (isSomeP TA) PA.
+    case TA': typechecks_tree => //=[env'] _.
+    rewrite typechecks_tree_big_and andbb.
+    admit.
+  case: ifP => //fA.
+    case PA: prune => //=[A'][<-]/=.
+    have:= HA _ _ _ _ (isSomeP TA) PA.
+    case TA': typechecks_tree => //=[env'] _.
+    rewrite typechecks_tree_big_and andbb.
+    admit.
+  move=> [<-]/=.
+  by rewrite TA/= TB TB0.
+Admitted.
+  
+
+Lemma tc_run p n s tree res env:
+  typechecks_tree p.(sig) env s tree ->
+  (exists b n', runT u p n s tree res b n') ->
+  match res with
+  | Zero => true
+  | One s => true
+  | Many s t => typechecks_tree p.(sig) env s t
+  end.
+Proof.
+  move=> +[b [n' H]].
+  elim_run H env => TA; only 2, 3: apply: IH.
+  - admit.
+  - admit.
+  - by apply: typechecks_tree_prune nA.
+  
+  elim_tree H.
+  elim
+  
+
+
+
+
+
+
